Removing tangle attractor yields valid subgame
Also:
- Every node in the graph outside of a tangle-attracted region still has successors not in that region.
- Rephrased alpha-maximality as being unable to extend the region.
- A player_tangle_subgraph is part of the whole graph (both nodes and edges)

More cleanup of the tangleattractors file will be needed later.

TangleAttractors.thy
@@ -11,26 +11,39 @@ context
   assumes fin_T: "finite T"
 begin
 
-subsection \<open>Tangle Attractors as an Inductive Predicate\<close>
 context
   fixes A :: "'v set"
 begin
+subsection \<open>Tangle Attractors as an Inductive Predicate\<close>
+(** Van Dijk defines a tangle attractor as an extension of the regular attractor. We define an
+    inductive predicate for a step of the attractor construction, which also constructs the strategy.
+    There are three cases:
+    own:
+    All vertices belonging to the player that have a successor in the previous step are added to the
+    attractor. The strategy is updated with an edge from it to that successor.
 
+    opponent:
+    All vertices belonging to the opponent that have only successors in the previous step are added
+    to the attractor. The strategy remains the same.
+
+    escape:
+    Every non-empty tangle belonging to the player in the set of known tangles that has escapes into
+    the previous step is added in its entirety to the attractor. For ease of proof we limit this to
+    only use attractors that are not already entirely inside the existing attractor. The strategy
+    is updated with the tangle strategy, but we omit the target set A from its domain. *)
 inductive tangle_attractor_step :: "'v set \<times> 'v strat \<Rightarrow> 'v set \<times> 'v strat \<Rightarrow> bool" where
   own: "\<lbrakk>x \<in> V\<^sub>\<alpha>-S; (x,y) \<in> E; y \<in> S\<rbrakk> \<Longrightarrow> tangle_attractor_step (S,\<sigma>) (insert x S,\<sigma>(x\<mapsto>y))"
 | opponent: "\<lbrakk>x \<in> V\<^sub>\<beta>-S; \<forall>y. (x,y) \<in> E \<longrightarrow> y \<in> S\<rbrakk> \<Longrightarrow> tangle_attractor_step (S,\<sigma>) (insert x S,\<sigma>)"
 | escape: "\<lbrakk>t \<in> T; t-S \<noteq> {}; opponent_escapes t \<noteq> {}; opponent_escapes t \<subseteq> S;
             player_tangle_strat t \<sigma>'\<rbrakk> \<Longrightarrow> tangle_attractor_step (S,\<sigma>) (S\<union>t,(\<sigma>' |` (t-A)) ++ \<sigma>)"
 
+(** The tangle attractor step is monotonous with respect to the set of vertices in the attracted
+    region. *)
 lemma tangle_attractor_step_mono: "tangle_attractor_step S S' \<Longrightarrow> fst S \<subset> fst S'"
   by (induction rule: tangle_attractor_step.induct) auto
 
-lemma tangle_attractor_step_rtranclp_mono: "tangle_attractor_step\<^sup>*\<^sup>* S S' \<Longrightarrow> fst S \<subseteq> fst S'"
-  apply (induction rule: rtranclp_induct)
-  subgoal by simp
-  subgoal using tangle_attractor_step_mono by blast
-  done
-
+(** The tangle attractor step's result is always in the union of the original attractor set and V.
+    This means that attractors to regions in V will be entirely in V. *)
 lemma tangle_attractor_step_ss: "tangle_attractor_step S S' \<Longrightarrow> fst S' \<subseteq> (fst S \<union> V)"
   apply (induction rule: tangle_attractor_step.induct)
   subgoal using V\<^sub>\<alpha>_subset by auto
@@ -38,31 +51,199 @@ lemma tangle_attractor_step_ss: "tangle_attractor_step S S' \<Longrightarrow> fs
   subgoal using tangles_T player_tangle_in_V by auto
   done
 
+(* If the original region is finite, then the region obtained in one step of the tangle attractor
+   is also finite. *)
+lemma fin_tangle_attractor_step: "tangle_attractor_step S S' \<Longrightarrow> finite (fst S) \<Longrightarrow> finite (fst S')"
+  using finite_subset[OF tangle_attractor_step_ss] by blast
+
+
+subsection \<open>Tangle Attractors\<close>
+(** We will be using the reflexive transitive closure of the step relation for our final definition.
+    To prove properties of the final definition, we will therefore need to prove them for the
+    reflexive transitive closure first. *)
+
+(** The reflexive transitive closure of steps is monotonous over the obtained region. This is less
+    strict than our monotonicity property for the individual steps because of the reflexivity. *)
+lemma tangle_attractor_step_rtranclp_mono: "tangle_attractor_step\<^sup>*\<^sup>* S S' \<Longrightarrow> fst S \<subseteq> fst S'"
+  apply (induction rule: rtranclp_induct)
+  subgoal by simp
+  subgoal using tangle_attractor_step_mono by blast
+  done
+
+(** The reflexive transitive closure of steps yields a subset of the union of the original set with
+    V. If we attract to a region in V, then the result will always be in V. *)
 lemma tangle_attractor_step_rtranclp_ss: "tangle_attractor_step\<^sup>*\<^sup>* S S' \<Longrightarrow> fst S' \<subseteq> (fst S \<union> V)"
   apply (induction rule: rtranclp_induct)
   subgoal by simp
   subgoal using tangle_attractor_step_ss by blast
   done
 
-lemma fin_tangle_attractor_step: "tangle_attractor_step S S' \<Longrightarrow> finite (fst S) \<Longrightarrow> finite (fst S')"
-  using finite_subset[OF tangle_attractor_step_ss] by blast
-
-lemma fin_tangle_attractor_step_rtranclp: "tangle_attractor_step\<^sup>*\<^sup>* S S' \<Longrightarrow> finite (fst S) \<Longrightarrow> finite (fst S')"
+(** The region in the result of the reflexive transitive closure of steps is finite if the original
+    set is finite. *)
+lemma fin_tangle_attractor_step_rtranclp: "tangle_attractor_step\<^sup>*\<^sup>* S S' \<Longrightarrow> finite (fst S)
+  \<Longrightarrow> finite (fst S')"
   using finite_subset[OF tangle_attractor_step_rtranclp_ss] by blast
 
-definition tangle_attractor_step_I :: "'v set \<times> 'v strat \<Rightarrow> bool" where
-  "tangle_attractor_step_I \<equiv> \<lambda>(S,\<sigma>).
+
+(** We finally get the definition for the attractor as a whole by taking the reflexive transitive
+    closure of the steps starting from the target set with an empty strategy. We also limit it to
+    only final results by saying it should not be in the domain of the relation; it cannot be
+    followed by another step. *)
+definition player_tangle_attractor :: "'v set \<Rightarrow> 'v strat \<Rightarrow> bool" where
+  "player_tangle_attractor X \<sigma> \<equiv> tangle_attractor_step\<^sup>*\<^sup>* (A,Map.empty) (X,\<sigma>) \<and>
+    \<not>Domainp tangle_attractor_step (X,\<sigma>)"
+
+(** The (inverse) reflexive transitive closure of the tangle attractor step is a well-founded
+    relation. *)
+lemma tangle_attractor_step_wf: "wfP (tangle_attractor_step\<inverse>\<inverse>)"
+  unfolding wfP_def
+  apply (rule wf_subset[of "inv_image (finite_psubset) (\<lambda>(s,\<sigma>). V - s)"]; clarsimp)
+  subgoal for S' \<sigma>' S \<sigma>
+    apply (erule tangle_attractor_step.cases)
+    subgoal using V\<^sub>\<alpha>_subset by blast
+    subgoal by auto
+    subgoal using player_tangle_in_V tangles_T by blast
+    done
+  done
+
+(** A wellfounded relation terminates. *)
+lemma wf_rel_terminates: "wfP R\<inverse>\<inverse> \<Longrightarrow> \<exists>X' \<sigma>'. R\<^sup>*\<^sup>* S (X',\<sigma>') \<and> \<not> Domainp R (X', \<sigma>')"
+  unfolding wfP_def
+  apply (induction S rule: wf_induct_rule)
+  subgoal for x apply (cases "Domainp R x"; clarsimp)
+    subgoal using converse_rtranclp_into_rtranclp[of R] by blast
+    subgoal using surj_pair[of x] by blast
+    done
+  done
+
+(** There always exists a tangle attractor. *)
+lemma player_tangle_attractor_exists: "\<exists>X \<sigma>. player_tangle_attractor X \<sigma>"
+  using wf_rel_terminates[OF tangle_attractor_step_wf]
+  unfolding player_tangle_attractor_def .
+
+(** Every node that is not in a tangle attractor still has successors outside of that attractor. *)
+lemma notin_player_tangle_attractor_succ:
+  "\<lbrakk>player_tangle_attractor X \<sigma>; v \<in> V; v \<notin> X\<rbrakk> \<Longrightarrow> E `` {v} - X \<noteq> {}"
+proof
+  assume attr: "player_tangle_attractor X \<sigma>" and
+         v_in_V: "v \<in> V" and
+         v_notin_X: "v \<notin> X" and
+         no_succs_outside_X: "E `` {v} - X = {}"
+  (** We need to unfold the definition of the attractor so we can use it for our induction later. *)
+  from attr have
+    attr_step_rtranclp: "tangle_attractor_step\<^sup>*\<^sup>* (A,Map.empty) (X,\<sigma>)" and
+    attr_step_result: "\<not>Domainp tangle_attractor_step (X,\<sigma>)"
+    unfolding player_tangle_attractor_def by auto
+
+  (** By our definition of a parity game, there must be successors to v. Furthermore, because we
+      have the assumption that there are no successors outside of X, all of them must be in X.
+      This also means that there exists at least one successor in X, which we will need for the case
+      that v belongs to the player. *)
+  from succ[OF v_in_V] have v_succ: "E `` {v} \<noteq> {}" .
+  with no_succs_outside_X v_in_V have all_succs_in_X: "\<forall>v'. (v,v') \<in> E \<longrightarrow> v' \<in> X" by blast
+  with v_succ have some_succ_in_X: "\<exists>v'. (v,v') \<in> E \<and> v' \<in> X" by blast
+
+  (** Now we have two cases: v belongs to the player, and v belongs to the opponent.
+      If v belongs to the player, and it has a successor in X, then it should be part of X by
+      the definition of our tangle attractor.
+      Likewise, if v belongs to the opponent, and all of its successors are in X, then it should
+      be part of X by the definition of the tangle attractor.
+      We have the assumption that v is not a part of X, so we have a contradiction, completing
+      our proof. *)
+  from v_in_V consider (v_player) "v \<in> V\<^sub>\<alpha>" | (v_opp) "v \<in> V\<^sub>\<beta>" by blast
+  thus "False"
+    using attr_step_rtranclp attr_step_result v_notin_X
+    apply cases
+    subgoal apply (induction rule: converse_rtranclp_induct)
+      using some_succ_in_X by (auto intro: tangle_attractor_step.own)
+    subgoal apply (induction rule: converse_rtranclp_induct)
+      using all_succs_in_X by (auto intro: tangle_attractor_step.opponent)
+    done
+qed
+
+(** The target of a tangle attractor is part of the attracted region. *)
+lemma target_in_player_tangle_attractor: "player_tangle_attractor X \<sigma> \<Longrightarrow> A \<subseteq> X"
+  unfolding player_tangle_attractor_def
+  using tangle_attractor_step_rtranclp_mono by fastforce
+
+(** An attracted region is a subset of the union of its target and V. This means that if the target
+    is in V, the attracted region is entirely in V. *)
+lemma player_tangle_attractor_ss: "player_tangle_attractor X \<sigma> \<Longrightarrow> X \<subseteq> A \<union> V"
+  unfolding player_tangle_attractor_def
+  using tangle_attractor_step_rtranclp_ss by fastforce
+
+(** If the target of the attractor is finite, so is the attracted region. *)
+lemma fin_player_tangle_attractor: "player_tangle_attractor X \<sigma> \<Longrightarrow> finite A \<Longrightarrow> finite X"
+  using finite_subset[OF player_tangle_attractor_ss] by blast
+
+
+subsubsection \<open>An Induction Rule for Tangle Attractors\<close>
+(** We want to define an induction rule for tangle attractors. To achieve this, we start with
+    an induction rule for the reflexive transitive closure of the tangle_attractor_step. *)
+lemma tangle_attractor_step_rtranclp_induct[consumes 1, case_names base own opponent escape]:
+  assumes tangle_attractor_step_rtranclp: "tangle_attractor_step\<^sup>*\<^sup>* S S'"
+  assumes base: "P S"
+  assumes own: "\<And>x S y \<sigma>. \<lbrakk>x \<in> V\<^sub>\<alpha>-S; (x,y) \<in> E; y \<in> S; P (S,\<sigma>)\<rbrakk> \<Longrightarrow> P (insert x S,\<sigma>(x\<mapsto>y))"
+  assumes opponent: "\<And>x S \<sigma>. \<lbrakk>x \<in> V\<^sub>\<beta>-S; \<forall>y. (x,y) \<in> E \<longrightarrow> y \<in> S; P (S,\<sigma>)\<rbrakk> \<Longrightarrow> P (insert x S,\<sigma>)"
+  assumes escape: "\<And>t S \<sigma>' \<sigma>. \<lbrakk>t \<in> T; t-S \<noteq> {}; opponent_escapes t \<noteq> {}; opponent_escapes t \<subseteq> S;
+                   player_tangle_strat t \<sigma>'; P (S,\<sigma>)\<rbrakk> \<Longrightarrow> P (S\<union>t, \<sigma>' |` (t-A) ++ \<sigma>)"
+  shows "P S'"
+  using tangle_attractor_step_rtranclp base
+proof (induction rule: rtranclp.induct)
+  case (rtrancl_refl S)
+  thus ?case by simp
+next
+  case (rtrancl_into_rtrancl S S' S'')
+  from this(2) this(3)[OF this(4)]
+  show ?case
+    apply (induction rule: tangle_attractor_step.induct)
+    subgoal using own by simp
+    subgoal using opponent by simp
+    subgoal using escape by simp
+    done
+qed
+
+(** We can now use this rule to make an induction rule for the tangle attractor itself.
+    This rule is internal, because it still depends on the assumptions of the context it is in. *)
+lemma player_tangle_attractor_induct_internal[consumes 1, case_names base own opponent escape]:
+  assumes attr: "player_tangle_attractor X \<sigma>"
+  assumes base: "P A Map.empty"
+  assumes own: "\<And>x S y \<sigma>. \<lbrakk>x \<in> V\<^sub>\<alpha>-S; (x,y) \<in> E; y \<in> S; P S \<sigma>\<rbrakk> \<Longrightarrow> P (insert x S) (\<sigma>(x\<mapsto>y))"
+  assumes opponent: "\<And>x S \<sigma>. \<lbrakk>x \<in> V\<^sub>\<beta> - S; \<forall>y. (x,y) \<in> E \<longrightarrow> y \<in> S; P S \<sigma>\<rbrakk> \<Longrightarrow> P (insert x S) \<sigma>"
+  assumes escape: "\<And>t S \<sigma>' \<sigma>. \<lbrakk>t \<in> T; t-S \<noteq> {}; opponent_escapes t \<noteq> {}; opponent_escapes t \<subseteq> S;
+                   player_tangle_strat t \<sigma>'; P S \<sigma>\<rbrakk> \<Longrightarrow> P (S\<union>t) (\<sigma>' |` (t-A) ++ \<sigma>)"
+  shows "P X \<sigma>"
+proof -
+  define P' :: "'v set \<times> 'v strat \<Rightarrow> bool" where "P' \<equiv> \<lambda>(a,b). P a b"
+  hence base': "P' (A,Map.empty)" and
+        own': "\<And>x S y \<sigma>. \<lbrakk>x \<in> V\<^sub>\<alpha>-S; (x,y) \<in> E; y \<in> S; P' (S,\<sigma>)\<rbrakk> \<Longrightarrow> P' (insert x S,\<sigma>(x\<mapsto>y))" and
+        opponent': "\<And>x S \<sigma>. \<lbrakk>x \<in> V\<^sub>\<beta>-S; \<forall>y. (x,y) \<in> E \<longrightarrow> y \<in> S; P' (S,\<sigma>)\<rbrakk> \<Longrightarrow> P' (insert x S,\<sigma>)" and
+        escape': "\<And>t S \<sigma>' \<sigma>. \<lbrakk>t \<in> T; t-S \<noteq> {}; opponent_escapes t \<noteq> {}; opponent_escapes t \<subseteq> S;
+                  player_tangle_strat t \<sigma>'; P' (S,\<sigma>)\<rbrakk> \<Longrightarrow> P' (S\<union>t,\<sigma>' |` (t-A) ++ \<sigma>)"
+    using base own opponent escape by auto
+  from attr have " tangle_attractor_step\<^sup>*\<^sup>* (A, \<lambda>x. None) (X, \<sigma>)"
+    unfolding player_tangle_attractor_def by blast
+  from this base' have "P' (X,\<sigma>)"
+    apply (induction rule: tangle_attractor_step_rtranclp_induct)
+    using own' opponent' escape' by auto
+  thus ?thesis
+    unfolding P'_def by simp
+qed
+
+subsection \<open>Tangle Attractor Strategies\<close>
+definition tangle_attractor_strat_I :: "'v set \<times> 'v strat \<Rightarrow> bool" where
+  "tangle_attractor_strat_I \<equiv> \<lambda>(S,\<sigma>).
    strategy_of V\<^sub>\<alpha> \<sigma> \<and> dom \<sigma> = V\<^sub>\<alpha> \<inter> (S-A) \<and> ran \<sigma> \<subseteq> S \<and>
    induced_subgraph V\<^sub>\<alpha> \<sigma> `` (S-A) \<subseteq> S \<and>
    (\<forall>x\<in>S. \<forall>xs ys. lasso_from_node (induced_subgraph V\<^sub>\<alpha> \<sigma>) x xs ys
       \<longrightarrow> (set (xs@ys) \<inter> A \<noteq> {} \<or> winning_player ys))"
 
-lemma tangle_attractor_step_I_base: "tangle_attractor_step_I (A,Map.empty)"
-  unfolding tangle_attractor_step_I_def using origin_in_lasso by fastforce
+lemma tangle_attractor_strat_I_base: "tangle_attractor_strat_I (A,Map.empty)"
+  unfolding tangle_attractor_strat_I_def using origin_in_lasso by fastforce
 
-lemma tangle_attractor_step_I_step:
-  "tangle_attractor_step S S' \<Longrightarrow> A \<subseteq> fst S \<Longrightarrow> tangle_attractor_step_I S
-   \<Longrightarrow> tangle_attractor_step_I S'"
+lemma tangle_attractor_strat_I_step:
+  "tangle_attractor_step S S' \<Longrightarrow> A \<subseteq> fst S \<Longrightarrow> tangle_attractor_strat_I S
+   \<Longrightarrow> tangle_attractor_strat_I S'"
 proof (induction rule: tangle_attractor_step.induct)
   case (own x S y \<sigma>)
   hence \<sigma>_strat: "strategy_of V\<^sub>\<alpha> \<sigma>" and
@@ -71,7 +252,7 @@ proof (induction rule: tangle_attractor_step.induct)
     \<sigma>_closed: "induced_subgraph V\<^sub>\<alpha> \<sigma> `` (S-A) \<subseteq> S" and
     \<sigma>_forces_A_or_wins: "\<forall>x\<in>S. \<forall>xs ys. lasso_from_node (induced_subgraph V\<^sub>\<alpha> \<sigma>) x xs ys
           \<longrightarrow> (set (xs@ys) \<inter> A \<noteq> {} \<or> winning_player ys)"
-    unfolding tangle_attractor_step_I_def by blast+
+    unfolding tangle_attractor_strat_I_def by blast+
   let ?S' = "insert x S"
   let ?\<sigma>' = "\<sigma>(x\<mapsto>y)"
 
@@ -152,7 +333,7 @@ proof (induction rule: tangle_attractor_step.induct)
   qed
 
   ultimately show ?case
-    unfolding tangle_attractor_step_I_def by blast
+    unfolding tangle_attractor_strat_I_def by blast
 
 next
   case (opponent x S \<sigma>)
@@ -162,7 +343,7 @@ next
     \<sigma>_closed_S: "induced_subgraph V\<^sub>\<alpha> \<sigma> `` (S-A) \<subseteq> S" and
     \<sigma>_forces_A_or_wins: "\<forall>x\<in>S. \<forall>xs ys. lasso_from_node (induced_subgraph V\<^sub>\<alpha> \<sigma>) x xs ys
           \<longrightarrow> (set (xs@ys) \<inter> A \<noteq> {} \<or> winning_player ys)"
-    unfolding tangle_attractor_step_I_def by blast+
+    unfolding tangle_attractor_strat_I_def by blast+
   let ?S' = "insert x S"
 
   from \<sigma>_closed_S opponent.hyps(2) have \<sigma>_closed_S': "induced_subgraph V\<^sub>\<alpha> \<sigma> `` (?S'-A) \<subseteq> ?S'"
@@ -227,7 +408,7 @@ next
   qed
 
   from \<sigma>_strat \<sigma>_dom \<sigma>_ran \<sigma>_closed_S' \<sigma>_forces_A_or_wins' opponent.hyps(1) show ?case
-    unfolding tangle_attractor_step_I_def by blast
+    unfolding tangle_attractor_strat_I_def by blast
 
 next
   case (escape t S \<sigma>' \<sigma>)
@@ -237,7 +418,7 @@ next
     \<sigma>_closed_S: "induced_subgraph V\<^sub>\<alpha> \<sigma> `` (S - A) \<subseteq> S" and
     \<sigma>_forces_A_or_wins: "\<forall>x\<in>S. \<forall>xs ys. lasso_from_node (induced_subgraph V\<^sub>\<alpha> \<sigma>) x xs ys
       \<longrightarrow> set (xs @ ys) \<inter> A \<noteq> {} \<or> winning_player ys"
-    unfolding tangle_attractor_step_I_def by auto
+    unfolding tangle_attractor_strat_I_def by auto
   let ?\<tau> = "(\<sigma>' |` (t-A)) ++ \<sigma>"
   let ?S' = "S\<union>t"
 
@@ -402,137 +583,105 @@ next
   qed
 
   from \<tau>_strat \<tau>_dom \<tau>_ran \<tau>_closed_S' \<tau>_forces_A_or_wins show ?case
-    unfolding tangle_attractor_step_I_def by blast
+    unfolding tangle_attractor_strat_I_def by blast
 qed
 
-lemma tangle_attractor_step_rtranclp_I:
-  "tangle_attractor_step\<^sup>*\<^sup>* S S' \<Longrightarrow> A \<subseteq> fst S \<Longrightarrow> tangle_attractor_step_I S \<Longrightarrow> tangle_attractor_step_I S'"
+(** The reflexive transitive closure of the tangle attractor step preserves the strategy invariant. *)
+lemma tangle_attractor_step_rtranclp_preserves_I:
+  "tangle_attractor_step\<^sup>*\<^sup>* S S' \<Longrightarrow> A \<subseteq> fst S \<Longrightarrow> tangle_attractor_strat_I S
+  \<Longrightarrow> tangle_attractor_strat_I S'"
   apply (induction rule: rtranclp_induct; simp)
-  using tangle_attractor_step_rtranclp_mono tangle_attractor_step_I_step subset_trans
+  using tangle_attractor_step_rtranclp_mono tangle_attractor_strat_I_step subset_trans
   by fast
 
-lemma tangle_attractor_step_wf: "wfP (tangle_attractor_step\<inverse>\<inverse>)"
-  unfolding wfP_def
-  apply (rule wf_subset[of "inv_image (finite_psubset) (\<lambda>(s,\<sigma>). V - s)"]; clarsimp)
-  subgoal for S' \<sigma>' S \<sigma>
-    apply (erule tangle_attractor_step.cases)
-    subgoal using V\<^sub>\<alpha>_subset by blast
-    subgoal by auto
-    subgoal using player_tangle_in_V tangles_T by blast
-    done
-  done
-
-lemma tangle_attractor_step_rtranclp_induct[consumes 1, case_names base own opponent escape]:
-  assumes tangle_attractor_step_rtranclp: "tangle_attractor_step\<^sup>*\<^sup>* S S'"
-  assumes base: "P S"
-  assumes own: "\<And>x S y \<sigma>. \<lbrakk>x \<in> V\<^sub>\<alpha>-S; (x,y) \<in> E; y \<in> S; P (S,\<sigma>)\<rbrakk> \<Longrightarrow> P (insert x S,\<sigma>(x\<mapsto>y))"
-  assumes opponent: "\<And>x S \<sigma>. \<lbrakk>x \<in> V\<^sub>\<beta>-S; \<forall>y. (x,y) \<in> E \<longrightarrow> y \<in> S; P (S,\<sigma>)\<rbrakk> \<Longrightarrow> P (insert x S,\<sigma>)"
-  assumes escape: "\<And>t S \<sigma>' \<sigma>. \<lbrakk>t \<in> T; t-S \<noteq> {}; opponent_escapes t \<noteq> {}; opponent_escapes t \<subseteq> S;
-                   player_tangle_strat t \<sigma>'; P (S,\<sigma>)\<rbrakk> \<Longrightarrow> P (S\<union>t, \<sigma>' |` (t-A) ++ \<sigma>)"
-  shows "P S'"
-  using tangle_attractor_step_rtranclp base
-proof (induction rule: rtranclp.induct)
-  case (rtrancl_refl S)
-  thus ?case by simp
-next
-  case (rtrancl_into_rtrancl S S' S'')
-  from this(2) this(3)[OF this(4)]
-  show ?case
-    apply (induction rule: tangle_attractor_step.induct)
-    subgoal using own by simp
-    subgoal using opponent by simp
-    subgoal using escape by simp
-    done
-qed
-
-(** Correctness check for the induction lemma *)
-lemma "tangle_attractor_step\<^sup>*\<^sup>* S S' \<Longrightarrow> finite (fst S) \<Longrightarrow> finite (fst S')"
-  apply (induction rule: tangle_attractor_step_rtranclp_induct)
-  subgoal by simp
-  subgoal by simp
-  subgoal by simp
-  subgoal using tangles_T fin_player_tangle by simp
-  done
-
-definition player_tangle_attractor :: "'v set \<Rightarrow> 'v strat \<Rightarrow> bool" where
-  "player_tangle_attractor X \<sigma> \<equiv> tangle_attractor_step\<^sup>*\<^sup>* (A,Map.empty) (X,\<sigma>)"
-
-lemma player_tangle_attractor_induct[consumes 1, case_names base own opponent escape]:
-  assumes attr: "player_tangle_attractor X \<sigma>"
-  assumes base: "P A Map.empty"
-  assumes own: "\<And>x S y \<sigma>. \<lbrakk>x \<in> V\<^sub>\<alpha>-S; (x,y) \<in> E; y \<in> S; P S \<sigma>\<rbrakk> \<Longrightarrow> P (insert x S) (\<sigma>(x\<mapsto>y))"
-  assumes opponent: "\<And>x S \<sigma>. \<lbrakk>x \<in> V\<^sub>\<beta> - S; \<forall>y. (x,y) \<in> E \<longrightarrow> y \<in> S; P S \<sigma>\<rbrakk> \<Longrightarrow> P (insert x S) \<sigma>"
-  assumes escape: "\<And>t S \<sigma>' \<sigma>. \<lbrakk>t \<in> T; t-S \<noteq> {}; opponent_escapes t \<noteq> {}; opponent_escapes t \<subseteq> S;
-                   player_tangle_strat t \<sigma>'; P S \<sigma>\<rbrakk> \<Longrightarrow> P (S\<union>t) (\<sigma>' |` (t-A) ++ \<sigma>)"
-  shows "P X \<sigma>"
-proof -
-  define P' :: "'v set \<times> 'v strat \<Rightarrow> bool" where "P' \<equiv> \<lambda>(a,b). P a b"
-  hence base': "P' (A,Map.empty)" and
-        own': "\<And>x S y \<sigma>. \<lbrakk>x \<in> V\<^sub>\<alpha>-S; (x,y) \<in> E; y \<in> S; P' (S,\<sigma>)\<rbrakk> \<Longrightarrow> P' (insert x S,\<sigma>(x\<mapsto>y))" and
-        opponent': "\<And>x S \<sigma>. \<lbrakk>x \<in> V\<^sub>\<beta>-S; \<forall>y. (x,y) \<in> E \<longrightarrow> y \<in> S; P' (S,\<sigma>)\<rbrakk> \<Longrightarrow> P' (insert x S,\<sigma>)" and
-        escape': "\<And>t S \<sigma>' \<sigma>. \<lbrakk>t \<in> T; t-S \<noteq> {}; opponent_escapes t \<noteq> {}; opponent_escapes t \<subseteq> S;
-                  player_tangle_strat t \<sigma>'; P' (S,\<sigma>)\<rbrakk> \<Longrightarrow> P' (S\<union>t,\<sigma>' |` (t-A) ++ \<sigma>)"
-    using base own opponent escape by auto
-  from attr base'
-  have "P' (X,\<sigma>)"
-    unfolding player_tangle_attractor_def
-    apply (induction rule: tangle_attractor_step_rtranclp_induct)
-    using own' opponent' escape' by auto
-  thus ?thesis
-    unfolding P'_def by simp
-qed
-
-lemma A_in_player_tangle_attractor: "player_tangle_attractor U \<sigma> \<Longrightarrow> A \<subseteq> U"
-  unfolding player_tangle_attractor_def
-  using tangle_attractor_step_rtranclp_mono by fastforce
-
-lemma player_tangle_attractor_ss: "player_tangle_attractor U \<sigma> \<Longrightarrow> U \<subseteq> A \<union> V"
-  unfolding player_tangle_attractor_def
-  using tangle_attractor_step_rtranclp_ss by fastforce
-
-lemma fin_player_tangle_attractor: "player_tangle_attractor U \<sigma> \<Longrightarrow> finite A \<Longrightarrow> finite U"
-  using finite_subset[OF player_tangle_attractor_ss] by blast
-
-lemma player_tangle_attractor_strat: "player_tangle_attractor U \<sigma> \<Longrightarrow>
-      strategy_of V\<^sub>\<alpha> \<sigma> \<and> dom \<sigma> = V\<^sub>\<alpha> \<inter> (U-A) \<and> ran \<sigma> \<subseteq> U \<and>
-      induced_subgraph V\<^sub>\<alpha> \<sigma> `` (U-A) \<subseteq> U \<and>
-      (\<forall>x\<in>U. \<forall>xs ys. lasso_from_node (induced_subgraph V\<^sub>\<alpha> \<sigma>) x xs ys
-        \<longrightarrow> set (xs @ ys) \<inter> A \<noteq> {} \<or> winning_player ys)"
-  using tangle_attractor_step_I_base tangle_attractor_step_rtranclp_I
-  unfolding player_tangle_attractor_def tangle_attractor_step_I_def
+(** The tangle attractor strategy belongs to the player, goes from V\<^sub>\<alpha>-A to X, is closed in X, and
+    forces all plays starting within it to either move to A, or be won by the player. *)
+lemma player_tangle_attractor_strat: "player_tangle_attractor X \<sigma> \<Longrightarrow>
+  strategy_of V\<^sub>\<alpha> \<sigma> \<and> dom \<sigma> = V\<^sub>\<alpha> \<inter> (X-A) \<and> ran \<sigma> \<subseteq> X \<and>
+  induced_subgraph V\<^sub>\<alpha> \<sigma> `` (X-A) \<subseteq> X \<and>
+  (\<forall>x\<in>X. \<forall>xs ys. lasso_from_node (induced_subgraph V\<^sub>\<alpha> \<sigma>) x xs ys
+    \<longrightarrow> set (xs @ ys) \<inter> A \<noteq> {} \<or> winning_player ys)"
+  using tangle_attractor_strat_I_base tangle_attractor_step_rtranclp_preserves_I
+  unfolding player_tangle_attractor_def tangle_attractor_strat_I_def
   by clarsimp
+
+find_theorems wf
+term lfp
+term mono
+thm wfP_induct_rule[OF tangle_attractor_step_wf]
+find_theorems mono
+find_theorems rtranclp Domainp
+lemma "\<lbrakk>tangle_attractor_step\<^sup>*\<^sup>* S S'; \<not>Domainp tangle_attractor_step S'; tangle_attractor_step\<^sup>*\<^sup>* S S''; \<not>Domainp tangle_attractor_step S''\<rbrakk> \<Longrightarrow> fst S' = fst S''"
+  sorry, xxx sorry
+term "(tangle_attractor_step\<^sup>*\<^sup>* S)"
+lemma "\<not>Domainp tangle_attractor_step\<^sup>*\<^sup>* S \<Longrightarrow> \<nexists>S'. tangle_attractor_step S S'"
+  by blast
+
+lemma a: "\<lbrakk>P\<^sup>*\<^sup>* A B; A\<noteq>B\<rbrakk> \<Longrightarrow> Rangep P B"
+  by (auto intro: rtranclp.cases)
+
+lemma b: "\<lbrakk>P\<^sup>*\<^sup>* A B; A\<noteq>B\<rbrakk> \<Longrightarrow> Domainp P A"
+  by (auto intro: converse_rtranclpE)
+
+lemma c: "\<lbrakk>\<not>Domainp P A; B\<noteq>A\<rbrakk> \<Longrightarrow> \<not>P\<^sup>*\<^sup>* A B"
+  by (auto intro: converse_rtranclpE)
+
+lemma tangle_attractor_step_set_comp: "tangle_attractor_step S S' \<Longrightarrow> fst S' \<subseteq>
+  (fst S
+   \<union> {x | x y. x \<in> V\<^sub>\<alpha>-fst S \<and> (x,y) \<in> E \<and> y \<in> fst S}
+   \<union> {x. x \<in> V\<^sub>\<beta>-fst S \<and> (\<forall>y. (x,y) \<in> E \<longrightarrow> y \<in> fst S)}
+   \<union> \<Union>{t. t \<in> T \<and> t - fst S \<noteq> {} \<and> opponent_escapes t \<noteq> {} \<and> opponent_escapes t \<subseteq> fst S})"
+  by (induction rule: tangle_attractor_step.induct) auto
+
+lemma tangle_attractor_step_set_membership: "\<lbrakk>tangle_attractor_step S S'; v \<in> fst S'\<rbrakk> \<Longrightarrow>
+  v \<in> fst S \<or>
+  (v \<in> V\<^sub>\<alpha>-fst S \<and> (\<exists>y. (v, y) \<in> E \<and> y \<in> fst S)) \<or>
+  (v \<in> V\<^sub>\<beta>-fst S \<and> (\<forall>y. (v, y) \<in> E \<longrightarrow> y \<in> fst S)) \<or>
+  (\<exists>t. v \<in> t \<and> t \<in> T \<and> t-fst S \<noteq> {} \<and> opponent_escapes t \<noteq> {} \<and> opponent_escapes t \<subseteq> fst S)"
+  using tangle_attractor_step_set_comp[of S S'] by blast
+
+lemma tangle_attractor_step_set_cases:
+  assumes "tangle_attractor_step S S'"
+  assumes "v \<in> fst S'"
+  obtains (base) "v \<in> fst S"
+        | (own) "v \<in> V\<^sub>\<alpha>-fst S \<and> (\<exists>y. (v, y) \<in> E \<and> y \<in> fst S)"
+        | (opponent)"v \<in> V\<^sub>\<beta>-fst S \<and> (\<forall>y. (v, y) \<in> E \<longrightarrow> y \<in> fst S)"
+        | (escape)"(\<exists>t. v \<in> t \<and> t \<in> T \<and> t-fst S \<noteq> {} \<and> opponent_escapes t \<noteq> {} \<and> opponent_escapes t \<subseteq> fst S)"
+  using tangle_attractor_step_set_membership[OF assms] by blast
 end (** End of context with fixed A *)
 
 
 subsection \<open>\<alpha>-maximal Regions\<close>
-(** A region is \<alpha>-maximal if it equals its tangle attractor. *)
+(** A region is \<alpha>-maximal if it equals its tangle attractor, i.e. TAttr(A) = A.
+    This definition is now clearly wrong - it needs changing! *)
 definition player_\<alpha>_max :: "'v set \<Rightarrow> bool" where
-  "player_\<alpha>_max A \<equiv> player_tangle_attractor A A Map.empty"
+  "player_\<alpha>_max A \<equiv> \<forall>\<sigma>. \<nexists>S'. tangle_attractor_step A (A,\<sigma>) S'" (** player_tangle_attractor A A Map.empty" *)
 
-lemma attracted_region_is_player_\<alpha>_max: "player_tangle_attractor A U \<sigma> \<Longrightarrow> player_\<alpha>_max U"
-  unfolding player_\<alpha>_max_def
-  apply (induction rule: player_tangle_attractor_induct)
-  subgoal unfolding player_tangle_attractor_def by blast
-  subgoal unfolding player_tangle_attractor_def by blast
-  subgoal unfolding player_tangle_attractor_def by blast
-  subgoal unfolding player_tangle_attractor_def by blast
-  done
+
+subsection \<open>\<alpha>-maximal Regions\<close>
+(** A region is \<alpha>-maximal if it equals its tangle attractor, i.e. TAttr(A) = A.
+    This definition is now clearly wrong - it needs changing! *)
+definition player_\<alpha>_max :: "'v set \<Rightarrow> bool" where
+  "player_\<alpha>_max A \<equiv> \<forall>\<sigma>. \<nexists>S'. tangle_attractor_step A (A,\<sigma>) S'" (** player_tangle_attractor A A Map.empty" *)
+
+(** Tangle attracted regions cannot be extended further with the tangle attractor. *)
+lemma attractor_no_extension:
+  "player_tangle_attractor A X \<sigma> \<Longrightarrow> \<nexists>S'. tangle_attractor_step A (X,\<sigma>) S'"
+  unfolding player_tangle_attractor_def by blast
+
+lemma attractor_no_extension':
+  "player_tangle_attractor A X \<sigma> \<Longrightarrow> \<nexists>S'. tangle_attractor_step X (X,Map.empty) S'"
+  unfolding player_tangle_attractor_def
+  apply (erule conjE)
+  apply (induction rule: rtranclp_induct)
+  sorry
 
 end (** End of context with fixed T *)
 
 (** We need this version of the induction lemma so we can supply the properties of T without losing
     our case names. *)
-lemma player_tangle_attractor_induct'[consumes 3, case_names base own opponent escape]:
-  assumes attr: "player_tangle_attractor T A X \<sigma>"
-  assumes tangles_T: "\<forall>t\<in>T. player_tangle t"
-  assumes fin_T: "finite T"
-  assumes base: "P A Map.empty"
-  assumes own: "\<And>x S y \<sigma>. \<lbrakk>x \<in> V\<^sub>\<alpha>-S; (x,y) \<in> E; y \<in> S; P S \<sigma>\<rbrakk> \<Longrightarrow> P (insert x S) (\<sigma>(x\<mapsto>y))"
-  assumes opponent: "\<And>x S \<sigma>. \<lbrakk>x \<in> V\<^sub>\<beta> - S; \<forall>y. (x,y) \<in> E \<longrightarrow> y \<in> S; P S \<sigma>\<rbrakk> \<Longrightarrow> P (insert x S) \<sigma>"
-  assumes escape: "\<And>t S \<sigma>' \<sigma>. \<lbrakk>t \<in> T; t-S \<noteq> {}; opponent_escapes t \<noteq> {}; opponent_escapes t \<subseteq> S;
-                   player_tangle_strat t \<sigma>'; P S \<sigma>\<rbrakk> \<Longrightarrow> P (S\<union>t) (\<sigma>' |` (t-A) ++ \<sigma>)"
-  shows "P X \<sigma>"
-  using player_tangle_attractor_induct[OF tangles_T fin_T attr] base own opponent escape by blast
+lemmas player_tangle_attractor_induct[consumes 3, case_names base own opponent escape] =
+  player_tangle_attractor_induct_internal
 
 end (** End of context player_paritygame *)
 
@@ -543,31 +692,76 @@ fun tangle_attractor :: "player \<Rightarrow> 'v set set \<Rightarrow> 'v set \<
   "tangle_attractor EVEN = P0.player_tangle_attractor"
 | "tangle_attractor ODD = P1.player_tangle_attractor"
 
-lemma A_in_tangle_attractor:
+lemma tangle_attractor_exists:
   assumes tangles_T: "\<forall>t\<in>T. tangle \<alpha> t"
   assumes fin_T: "finite T"
-  shows "tangle_attractor \<alpha> T A U \<sigma> \<Longrightarrow> A \<subseteq> U"
-  using assms P0.A_in_player_tangle_attractor P1.A_in_player_tangle_attractor
+  shows "\<exists>X \<sigma>. tangle_attractor \<alpha> T A X \<sigma>"
+  using assms P0.player_tangle_attractor_exists P1.player_tangle_attractor_exists
+  by (cases \<alpha>; simp)
+
+lemma notin_tangle_attractor_succ:
+  assumes tangles_T: "\<forall>t\<in>T. tangle \<alpha> t"
+  assumes fin_T: "finite T"
+  shows "\<lbrakk>tangle_attractor \<alpha> T A X \<sigma>; v \<in> V; v \<notin> X\<rbrakk> \<Longrightarrow> E `` {v}-X \<noteq> {}"
+  using assms P0.notin_player_tangle_attractor_succ P1.notin_player_tangle_attractor_succ
+  by(cases \<alpha>; simp)
+
+lemma target_in_tangle_attractor:
+  assumes tangles_T: "\<forall>t\<in>T. tangle \<alpha> t"
+  assumes fin_T: "finite T"
+  shows "tangle_attractor \<alpha> T A X \<sigma> \<Longrightarrow> A \<subseteq> X"
+  using assms P0.target_in_player_tangle_attractor P1.target_in_player_tangle_attractor
   by (cases \<alpha>; simp)
 
 lemma tangle_attractor_ss:
   assumes tangles_T: "\<forall>t\<in>T. tangle \<alpha> t"
   assumes fin_T: "finite T"
-  shows "tangle_attractor \<alpha> T A U \<sigma> \<Longrightarrow> U \<subseteq> A \<union> V"
+  shows "tangle_attractor \<alpha> T A X \<sigma> \<Longrightarrow> X \<subseteq> A \<union> V"
   using assms P0.player_tangle_attractor_ss P1.player_tangle_attractor_ss
   by (cases \<alpha>; simp)
 
 lemma tangle_attractor_strat:
   assumes tangles_T: "\<forall>t\<in>T. tangle \<alpha> t"
   assumes fin_T: "finite T"
-  shows "tangle_attractor \<alpha> T A U \<sigma> \<Longrightarrow>
-         strategy_of_player \<alpha> \<sigma> \<and> dom \<sigma> = V_player \<alpha> \<inter> (U-A) \<and> ran \<sigma> \<subseteq> U \<and>
-         induced_subgraph (V_player \<alpha>) \<sigma> `` (U-A) \<subseteq> U \<and>
-         (\<forall>x\<in>U. \<forall>xs ys. lasso_from_node (induced_subgraph (V_player \<alpha>) \<sigma>) x xs ys
+  shows "tangle_attractor \<alpha> T A X \<sigma> \<Longrightarrow>
+         strategy_of_player \<alpha> \<sigma> \<and> dom \<sigma> = V_player \<alpha> \<inter> (X-A) \<and> ran \<sigma> \<subseteq> X \<and>
+         induced_subgraph (V_player \<alpha>) \<sigma> `` (X-A) \<subseteq> X \<and>
+         (\<forall>x\<in>X. \<forall>xs ys. lasso_from_node (induced_subgraph (V_player \<alpha>) \<sigma>) x xs ys
             \<longrightarrow> set (xs @ ys) \<inter> A \<noteq> {} \<or> player_wins_list \<alpha> ys)"
   unfolding strategy_of_player_def
   using assms P0.player_tangle_attractor_strat P1.player_tangle_attractor_strat
   by (cases \<alpha>; simp add: V\<^sub>1_def)
+
+lemma fin_tangle_attractor:
+  assumes tangles_T: "\<forall>t\<in>T. tangle \<alpha> t"
+  assumes fin_T: "finite T"
+  shows "tangle_attractor \<alpha> T A X \<sigma> \<Longrightarrow> finite A \<Longrightarrow> finite X"
+  using assms P0.fin_player_tangle_attractor P1.fin_player_tangle_attractor
+  by (cases \<alpha>; simp)
+
+(** If you remove a tangle attractor from the game, the resulting graph is a valid subgame. *)
+lemma remove_tangle_attractor_subgame:
+  assumes tangles_T: "\<forall>t\<in>T. tangle \<alpha> t"
+  assumes fin_T: "finite T"
+  assumes tangle_attractor: "tangle_attractor \<alpha> T A X \<sigma>"
+  shows "paritygame (Restr E (V-X)) (V-X) (V\<^sub>0-X)"
+proof (unfold_locales)
+  show " Restr E (V-X) \<subseteq> (V-X)\<times>(V-X)" by blast
+  show "finite (V-X)" by simp
+  show "V\<^sub>0-X \<subseteq> V-X" using V\<^sub>0_in_V by blast
+  show "\<And>v. v \<in> V-X \<Longrightarrow> Restr E (V-X) `` {v} \<noteq> {}"
+  proof -
+    fix v
+    assume v_in_V_min_X: "v \<in> V-X"
+    hence v_in_V: "v\<in>V" by simp
+    from v_in_V_min_X have "v \<notin> X" by simp
+    with notin_tangle_attractor_succ[OF tangles_T fin_T tangle_attractor v_in_V]
+    have "E `` {v} - X \<noteq> {}" by simp
+    then obtain w where w: "(v,w) \<in> E \<and> w \<in> V-X" using E_in_V by blast
+    with v_in_V_min_X have "(v,w) \<in> Restr E (V-X)" using E_in_V by blast
+    then show "Restr E (V-X) `` {v} \<noteq> {}" by blast
+  qed
+qed
 
 subsection \<open>\<alpha>-maximal regions\<close>
 fun \<alpha>_max :: "player \<Rightarrow> 'v set set \<Rightarrow> 'v set \<Rightarrow> bool" where
